Structural substitution overhaul. Checkpoint.

theories/Hole.v
@@ -1,48 +1,95 @@
 From Lang Require Import
+  Invert
   Terms.
 
 Inductive hole : Set :=
   | HoleHere
-  | HolePackTy (id : string) (arg : option string) (curry : term)
-  | HolePackCurry (id : string) (arg : option string) (ty : term)
-  | HoleForATy (arg : option string) (body : term)
-  | HoleForABody (arg : option string) (ty : term)
-  | HoleApplF (x : term)
-  | HoleApplX (f : term)
+  | HolePackTy (id : string) (arg : option string) (ty : hole) (curry : term)
+  | HolePackCurry (id : string) (arg : option string) (ty : term) (curry : hole)
+  | HoleForATy (arg : option string) (ty : hole) (body : term)
+  | HoleForABody (arg : option string) (ty : term) (body : hole)
+  | HoleApplF (f : hole) (x : term)
+  | HoleApplX (f : term) (x : hole)
   .
 
-Definition fill : hole -> term -> term := fun h t =>
+Fixpoint fill h t : term :=
   match h with
   | HoleHere => t
-  | HolePackTy id arg curry => TmPack id arg t curry
-  | HolePackCurry id arg ty => TmPack id arg ty t
-  | HoleForATy arg body => TmForA arg t body
-  | HoleForABody arg ty => TmForA arg ty t
-  | HoleApplF x => TmAppl t x
-  | HoleApplX f => TmAppl f t
+  | HolePackTy id arg ty curry => TmPack id arg (fill ty t) curry
+  | HolePackCurry id arg ty curry => TmPack id arg ty (fill curry t)
+  | HoleForATy arg ty body => TmForA arg (fill ty t) body
+  | HoleForABody arg ty body => TmForA arg ty (fill body t)
+  | HoleApplF f x => TmAppl (fill f t) x
+  | HoleApplX f x => TmAppl f (fill x t)
   end.
 
 Inductive Fill : hole -> term -> term -> Prop :=
   | FillHere : forall t,
       Fill HoleHere t t
-  | FillPackTy : forall id arg ty curry,
-      Fill (HolePackTy id arg curry) ty (TmPack id arg ty curry)
-  | FillPackCurry : forall id arg ty curry,
-      Fill (HolePackCurry id arg ty) curry (TmPack id arg ty curry)
-  | FillForATy : forall arg ty body,
-      Fill (HoleForATy arg body) ty (TmForA arg ty body)
-  | FillForABody : forall arg ty body,
-      Fill (HoleForABody arg ty) body (TmForA arg ty body)
-  | FillApplF : forall f x,
-      Fill (HoleApplF x) f (TmAppl f x)
-  | FillApplX : forall f x,
-      Fill (HoleApplX f) x (TmAppl f x)
+  | FillPackTy : forall t id arg ty curry ty',
+      Fill ty t ty' ->
+      Fill (HolePackTy id arg ty curry) t (TmPack id arg ty' curry)
+  | FillPackCurry : forall t id arg ty curry curry',
+      Fill curry t curry' ->
+      Fill (HolePackCurry id arg ty curry) t (TmPack id arg ty curry')
+  | FillForATy : forall t arg ty body ty',
+      Fill ty t ty' ->
+      Fill (HoleForATy arg ty body) t (TmForA arg ty' body)
+  | FillForABody : forall t arg ty body body',
+      Fill body t body' ->
+      Fill (HoleForABody arg ty body) t (TmForA arg ty body')
+  | FillApplF : forall t f x f',
+      Fill f t f' ->
+      Fill (HoleApplF f x) t (TmAppl f' x)
+  | FillApplX : forall t f x x',
+      Fill x t x' ->
+      Fill (HoleApplX f x) t (TmAppl f x')
   .
 
 Theorem reflect_fill : forall h t t',
   fill h t = t' <-> Fill h t t'.
 Proof.
   split; intros.
-  - destruct h; subst; constructor.
-  - destruct H; reflexivity.
+  - generalize dependent t. generalize dependent t'.
+    induction h; intros; subst; simpl in *; constructor; apply IHh; reflexivity.
+  - induction H; simpl in *; try rewrite IHFill; reflexivity.
+Qed.
+
+Fixpoint eq_hole a b :=
+  match a, b with
+  | HoleHere, HoleHere =>
+      true
+  | HolePackTy ida arga tya currya, HolePackTy idb argb tyb curryb =>
+      andb (eqb ida idb) (andb (eq_opt arga argb) (andb (eq_hole tya tyb) (eq_term currya curryb)))
+  | HolePackCurry ida arga tya currya, HolePackCurry idb argb tyb curryb =>
+      andb (eqb ida idb) (andb (eq_opt arga argb) (andb (eq_term tya tyb) (eq_hole currya curryb)))
+  | HoleForATy arga tya currya, HoleForATy argb tyb curryb =>
+      andb (eq_opt arga argb) (andb (eq_hole tya tyb) (eq_term currya curryb))
+  | HoleForABody arga tya currya, HoleForABody argb tyb curryb =>
+      andb (eq_opt arga argb) (andb (eq_term tya tyb) (eq_hole currya curryb))
+  | HoleApplF fa xa, HoleApplF fb xb =>
+      andb (eq_hole fa fb) (eq_term xa xb)
+  | HoleApplX fa xa, HoleApplX fb xb =>
+      andb (eq_term fa fb) (eq_hole xa xb)
+  | _, _ => false
+  end.
+
+Ltac rf n := constructor; intros C; invert C; apply n; reflexivity.
+Theorem eq_hole_spec : forall a b,
+  Bool.reflect (a = b) (eq_hole a b).
+Proof.
+  induction a; intros []; simpl in *; try solve [constructor; try reflexivity; try (intro C; discriminate C)];
+  try (destruct (eqb_spec id id0); [| rf n]);
+  try (destruct (eq_opt_spec arg arg0); [| rf n]);
+  try (destruct (IHa ty); [| rf n]);
+  try (destruct (eq_term_spec curry curry0); [| rf n]);
+  try (destruct (eq_term_spec ty ty0); [| rf n]);
+  try (destruct (IHa curry); [| rf n]);
+  try (destruct (eq_term_spec body body0); [| rf n]);
+  try (destruct (IHa body); [| rf n]);
+  try (destruct (IHa f); [| rf n]);
+  try (destruct (eq_term_spec x x0); [| rf n]);
+  try (destruct (eq_term_spec f f0); [| rf n]);
+  try (destruct (IHa x); [| rf n]);
+  constructor; subst; reflexivity.
 Qed.
