theories/StructuralSubst.v
@@ -3,35 +3,36 @@ From Coq Require Export
 Export ListNotations.
 From Lang Require Import
   FstCmp
+  StructuralHole
   Invert
   StructuralFreeVariables
   Terms.
 
-Fixpoint smap
-  (f : (term -> term) -> term -> term)
-  (x : list (string * (term -> term))) :
-  list (string * (term -> term)) :=
+Fixpoint smap {A B}
+  (f : B -> B)
+  (x : list (A * B)) :
+  list (A * B) :=
   match x with
   | [] => []
   | (s, g) :: tl => (s, f g) :: smap f tl
   end.
 
-Theorem smap_distr : forall f a b,
-  smap f (a ++ b) = smap f a ++ smap f b.
+Theorem smap_distr : forall {A B} f a b,
+  @smap A B f (a ++ b) = smap f a ++ smap f b.
 Proof.
-  intros f a. generalize dependent f. induction a; intros; simpl in *.
+  intros A B f a. generalize dependent f. induction a; intros; simpl in *.
   { reflexivity. } destruct a. rewrite IHa. reflexivity.
 Qed.
 
-Theorem smap_len : forall f li,
-  Datatypes.length (smap f li) = Datatypes.length li.
+Theorem smap_len : forall {A B} f li,
+  Datatypes.length (@smap A B f li) = Datatypes.length li.
 Proof.
-  intros f li. generalize dependent f. induction li; intros; simpl in *.
+  intros A B f li. generalize dependent f. induction li; intros; simpl in *.
   { reflexivity. } destruct a. simpl. rewrite IHli. reflexivity.
 Qed.
 
-Theorem map_fst_smap : forall f li,
-  map fst (smap f li) = map fst li.
+Theorem map_fst_smap : forall {A B} f li,
+  map fst (@smap A B f li) = map fst li.
 Proof. induction li. { reflexivity. } destruct a. simpl. rewrite IHli. reflexivity. Qed.
 
 Fixpoint remove_key_all {T} x (li : list (string * T)) :=
@@ -58,121 +59,65 @@ Proof.
   rewrite eqb_sym in H1. rewrite H1. f_equal. apply IHli. assumption.
 Qed.
 
-(* Ludicrous that this is the easiest correct definition to write.
- * Generates substitution functions for every free variable at once. *)
-Fixpoint structural_grand_unified_subst t : list (string * (term -> term)) :=
+Fixpoint fold_rm_acc {A B} out (pred : A -> bool) (f : A -> B -> B) acc li :=
+  match li with
+  | [] => (acc, out)
+  | hd :: tl =>
+      if pred hd then
+        fold_rm_acc out pred f (f hd acc) tl
+      else
+        fold_rm_acc (hd :: out) pred f acc tl
+  end.
+Definition fold_rm {A B} := @fold_rm_acc A B [].
+Arguments fold_rm {A B}/ pred f acc li.
+
+Fixpoint structural_subst_hole x t :=
   match t with
   | TmVoid
   | TmStar _
   | TmAtom _ =>
-      []
-  | TmVarS s =>
-      [(s, fun x => x)]
+      SHoleTerm t
+  | TmVarS z =>
+      if eqb z x then SHoleHere else SHoleTerm t
   | TmPack id arg ty curry =>
-      smap (fun f x => TmPack id arg (f x) curry) (structural_grand_unified_subst ty) ++
-      smap (fun f x => TmPack id arg ty (f x)) (
-        let recursed := structural_grand_unified_subst curry in
-        match arg with
-        | None => recursed
-        | Some a => remove_key_all a recursed
-        end)
+      SHolePack id arg (structural_subst_hole x ty) (
+        if eq_opt arg (Some x) then
+          SHoleTerm curry
+        else
+          structural_subst_hole x curry)
   | TmForA arg ty body =>
-      smap (fun f x => TmForA arg (f x) body) (structural_grand_unified_subst ty) ++
-      smap (fun f x => TmForA arg ty (f x)) (
-        let recursed := structural_grand_unified_subst body in
-        match arg with
-        | None => recursed
-        | Some a => remove_key_all a recursed
-        end)
-  | TmAppl a b =>
-      smap (fun f x => TmAppl (f x) b) (structural_grand_unified_subst a) ++
-      smap (fun f x => TmAppl a (f x)) (structural_grand_unified_subst b)
+      SHoleForA arg (structural_subst_hole x ty) (
+        if eq_opt arg (Some x) then
+          SHoleTerm body
+        else
+          structural_subst_hole x body)
+  | TmAppl f z =>
+      SHoleAppl (structural_subst_hole x f) (structural_subst_hole x z)
   end.
+Definition structural_subst x y t := sfill (structural_subst_hole x t) y.
+Arguments structural_subst/ x y t.
 
-Fixpoint pair_lookup {V} key (pairs : list (string * V)) :=
-  match pairs with
-  | [] => None
-  | (k, v) :: tl => if eqb key k then Some v else pair_lookup key tl
-  end.
+Example structural_subst_simple : forall f repl x, x <> f ->
+  structural_subst f repl (TmAppl (TmVarS f) (TmVarS x)) = (TmAppl repl (TmVarS x)).
+Proof. intros. simpl. rewrite eqb_refl. apply eqb_neq in H. rewrite H. reflexivity. Qed.
 
-Definition structural_subst x y t := option_map (fun f => f y) (pair_lookup x (structural_grand_unified_subst t)).
-Arguments structural_subst x y t/.
-
-Example structural_subst_simple : forall f x,
-  structural_subst f TmVoid (TmAppl (TmVarS f) x) = Some (TmAppl TmVoid x).
+Example structural_subst_shadowing : forall x y,
+  structural_subst x y (TmForA (Some x) TmVoid (TmVarS x)) = TmForA (Some x) TmVoid (TmVarS x). (* unchanged *)
 Proof. intros. simpl. rewrite eqb_refl. reflexivity. Qed.
 
-Example structural_grand_unified_subst_simple :
-  structural_grand_unified_subst (TmAppl (TmVarS "f"%string) (TmVarS "x"%string)) = [
-    ("f"%string, fun t => TmAppl t (TmVarS "x"%string));
-    ("x"%string, fun t => TmAppl (TmVarS "f"%string) t)].
-Proof. reflexivity. Qed.
-
-Example structural_grand_unified_subst_lambda :
-  structural_grand_unified_subst (TmForA (Some "x") (TmVarS "T") (TmAppl (TmVarS "x") (TmVarS "x")))%string = [
-    ("T", fun x => TmForA (Some "x") x (TmAppl (TmVarS "x") (TmVarS "x")))]%string.
-    (* do NOT ignore the first `x`, unlike the non-structural version, even thoguh it's bound *)
-Proof. reflexivity. Qed.
+Example structural_subst_not_shadowing : forall x y z, z <> x ->
+  structural_subst x y (TmForA (Some z) TmVoid (TmVarS x)) = TmForA (Some z) TmVoid y. (* changed *)
+Proof. intros. simpl. rewrite eqb_refl. apply eqb_neq in H. rewrite H. reflexivity. Qed.
 
 Lemma fst_cmp_eqb : forall {T} a a' b b',
   @fst_cmp T T (a, b) (a', b') = eqb a a'.
 Proof. reflexivity. Qed.
 
-Theorem structural_grand_unified_subst_fv : forall t,
-  structural_fv t = map fst (structural_grand_unified_subst t).
-Proof.
-  induction t; intros; subst; simpl in *; try reflexivity; repeat rewrite slow_down;
-  repeat rewrite IHt1; repeat rewrite IHt2; repeat rewrite map_distr; repeat rewrite map_fst_smap; [| | reflexivity];
-  destruct arg; f_equal; repeat rewrite <- partition_pf_fast_slow; try rewrite (map_fst_partition_pf _ _ _ _ fst_cmp_eqb);
-  repeat rewrite map_fst_smap; repeat rewrite remove_all_key_eq; reflexivity.
-Qed.
-
-Lemma pair_lookup_smap : forall f x li,
-  pair_lookup x (smap f li) = option_map f (pair_lookup x li).
-Proof.
-  intros f x li. generalize dependent x. generalize dependent f.
-  induction li; intros; simpl in *. { reflexivity. }
-  destruct a. simpl. destruct (eqb x s) eqn:E. { reflexivity. } apply IHli.
-Qed.
-
-Lemma pair_lookup_app : forall {T} x a b,
-  @pair_lookup T x (a ++ b) =
-  match pair_lookup x a with
-  | None => pair_lookup x b
-  | Some out => Some out
-  end.
-Proof.
-  intros T x a. generalize dependent x. induction a; intros; simpl in *. { reflexivity. }
-  destruct a. destruct (eqb x s). { reflexivity. } apply IHa.
-Qed.
-
-Lemma pair_lookup_Forall_snd : forall {T} P li x y,
-  Forall P (map snd li) ->
-  @pair_lookup T x li = Some y ->
-  P y.
-Proof.
-  intros T P li x y Hf Hl. generalize dependent y. generalize dependent x.
-  remember (map snd li) eqn:Emap. generalize dependent li.
-  induction Hf; intros; destruct li; invert Emap; try discriminate Hl.
-  destruct p. simpl in *. destruct (eqb x0 s) eqn:E. { invert Hl. assumption. }
-  eapply IHHf; [reflexivity |]. apply Hl.
-Qed.
-
-Lemma pair_lookup_Forall : forall {T} P li x t,
-  Forall P li ->
-  @pair_lookup T x li = Some t ->
-  P (x, t).
-Proof.
-  intros T P li x t Hf Hl. generalize dependent t. generalize dependent x.
-  induction Hf; intros; simpl in *. { discriminate Hl. } destruct x as [k v].
-  destruct (eqb x0 k) eqn:E; [apply eqb_eq in E; invert Hl | apply IHHf]; assumption.
-Qed.
-
-Theorem Forall_smap : forall f P li,
-  Forall (fun p : _ * _ => let (x, g) := p in P (x, f g)) li ->
+Theorem Forall_smap : forall {A B} f P li,
+  Forall (fun p : A * B => let (x, g) := p in P (x, f g)) li ->
   Forall P (smap f li).
 Proof.
-  intros. remember (fun p : string * (term -> term) => let (x, g) := p in P (x, f g)) as F eqn:EF.
+  intros. remember (fun p : _ * _ => let (x, g) := p in P (x, f g)) as F eqn:EF.
   generalize dependent P. generalize dependent f. induction H; intros; [apply Forall_nil |].
   destruct x as [s g]. subst. simpl in *. constructor; [assumption |]. apply IHForall. reflexivity.
 Qed.
@@ -212,31 +157,76 @@ Proof.
   unfold fst_cmp. simpl. apply eqb_neq in n. rewrite n. apply (IHli _ t).
 Qed.
 
-(*
-Theorem incl_partition_pf_fst : forall {T} hi lo,
-  incl (@partition_pf_slow (string * T) fst_cmp hi lo) hi.
+Theorem structural_subst_id : forall x t,
+  structural_subst x (TmVarS x) t = t.
 Proof.
-  unfold incl. induction hi; intros; simpl in *. { destruct H. }
-  destruct (existsb (fst_cmp a) lo) eqn:El; simpl in *. { right. apply (IHhi _ _ H). }
-  destruct (existsb (fst_cmp a) hi) eqn:Eh; simpl in *. { right. apply (IHhi _ _ H). }
-  destruct a as [k1 v1]. destruct a0 as [k2 v2]. destruct H; [| right; apply (IHhi _ _ H)].
-  left. assumption.
-Qed.
-*)
-
-Theorem structural_grand_unified_subst_id : forall t,
-  let P := fun p : _ * _ => let (x, f) := p in f (TmVarS x) = t in
-  Forall P (structural_grand_unified_subst t).
-Proof.
-  induction t as [| | | | id arg a IHa b IHb | arg a IHa b IHb | a IHa b IHb]; simpl in *; repeat constructor;
-  apply Forall_app; split; apply Forall_smap; try (destruct arg; [eapply incl_Forall; [apply remove_key_all_incl |] |]);
-  (eapply Forall_impl; [| try apply IHa; apply IHb]); intros; destruct a0; rewrite H; reflexivity.
+  intros. generalize dependent x. induction t; intros; simpl in *; try reflexivity.
+  - destruct (eqb_spec id x); subst; reflexivity.
+  - destruct (eq_opt_spec arg (Some x)); subst; simpl in *; rewrite IHt1; [| rewrite IHt2]; reflexivity.
+  - destruct (eq_opt_spec arg (Some x)); subst; simpl in *; rewrite IHt1; [| rewrite IHt2]; reflexivity.
+  - rewrite IHt1. rewrite IHt2. reflexivity.
 Qed.
 
-Theorem structural_subst_id : forall x t s,
-  structural_subst x (TmVarS x) t = Some s ->
-  s = t.
+Theorem structural_subst_fv : forall x y t,
+  ~In x (structural_fv y) ->
+  ~In x (structural_fv (structural_subst x y t)).
 Proof.
-  intros. unfold structural_subst in *. destruct (pair_lookup x (structural_grand_unified_subst t)) eqn:Ep; invert H.
-  eapply pair_lookup_Forall in Ep; [| apply structural_grand_unified_subst_id]. assumption.
+  intros. generalize dependent x. generalize dependent y. induction t; intros; simpl in *; intro C; try solve [destruct C];
+  [destruct (eqb_spec id x); subst; simpl in *; [apply H in C as [] |]; destruct C; [| destruct H0]; apply n; assumption | | |];
+  specialize (IHt1 _ _ H); specialize (IHt2 _ _ H); try destruct arg; apply in_app_iff in C as [C | C];
+  try apply IHt1 in C as []; try apply IHt2 in C as []; simpl in *;
+  (destruct (eqb_spec s x); [subst; eapply in_remove_all; apply C |]);
+  (apply in_remove_all_neq in C; [| intro E; subst; apply n; reflexivity]); apply IHt2 in C as [].
+Qed.
+
+Inductive StructuralSubst (x : string) : term -> structural_hole -> Prop :=
+  | SSubstVoid :
+      StructuralSubst x TmVoid (SHoleTerm TmVoid)
+  | SSubstStar : forall univ,
+      StructuralSubst x (TmStar univ) (SHoleTerm (TmStar univ))
+  | SSubstVarSEq :
+      StructuralSubst x (TmVarS x) SHoleHere
+  | SSubstVarSNEq : forall y,
+      x <> y ->
+      StructuralSubst x (TmVarS y) (SHoleTerm (TmVarS y))
+  | SSubstAtom : forall id,
+      StructuralSubst x (TmAtom id) (SHoleTerm (TmAtom id))
+  | SSubstPackShadow : forall id ty curry ty',
+      StructuralSubst x ty ty' ->
+      StructuralSubst x (TmPack id (Some x) ty curry) (SHolePack id (Some x) ty' (SHoleTerm curry))
+  | SSubstPack : forall id arg ty curry ty' curry',
+      arg <> Some x ->
+      StructuralSubst x ty ty' ->
+      StructuralSubst x curry curry' ->
+      StructuralSubst x (TmPack id arg ty curry) (SHolePack id arg ty' curry')
+  | SSubstForAShadow : forall ty body ty',
+      StructuralSubst x ty ty' ->
+      StructuralSubst x (TmForA (Some x) ty body) (SHoleForA (Some x) ty' (SHoleTerm body))
+  | SSubstForA : forall arg ty body ty' body',
+      arg <> Some x ->
+      StructuralSubst x ty ty' ->
+      StructuralSubst x body body' ->
+      StructuralSubst x (TmForA arg ty body) (SHoleForA arg ty' body')
+  | SSubstAppl : forall f z f' z',
+      StructuralSubst x f f' ->
+      StructuralSubst x z z' ->
+      StructuralSubst x (TmAppl f z) (SHoleAppl f' z')
+  .
+
+Theorem reflect_structural_subst : forall x t h,
+  structural_subst_hole x t = h <-> StructuralSubst x t h.
+Proof.
+  split; intros.
+  - generalize dependent x. generalize dependent h. induction t; intros; subst; simpl in *; try solve [constructor].
+    + destruct (eqb_spec id x). { subst. constructor. } constructor. intro C. subst. apply n. reflexivity.
+    + destruct (eq_opt_spec arg (Some x)). { subst. constructor. apply IHt1. reflexivity. }
+      constructor; [assumption | apply IHt1 | apply IHt2]; reflexivity.
+    + destruct (eq_opt_spec arg (Some x)). { subst. constructor. apply IHt1. reflexivity. }
+      constructor; [assumption | apply IHt1 | apply IHt2]; reflexivity.
+    + constructor; [apply IHt1 | apply IHt2]; reflexivity.
+  - induction H; simpl in *; try rewrite eqb_refl; try rewrite IHStructuralSubst;
+    try rewrite IHStructuralSubst1; try rewrite IHStructuralSubst2; try reflexivity.
+    + apply eqb_neq in H. rewrite eqb_sym in H. rewrite H. reflexivity.
+    + destruct (eq_opt_spec arg (Some x)). { subst. contradiction H. reflexivity. } reflexivity.
+    + destruct (eq_opt_spec arg (Some x)). { subst. contradiction H. reflexivity. } reflexivity.
 Qed.
