theories/Subst.v
@@ -4,8 +4,10 @@ Export ListNotations.
 From Lang Require Import
   FreeVariables
   FstCmp
+  Hole
   Invert
   Partition
+  PartitionKV
   StructuralFreeVariables
   StructuralSubst
   Terms.
@@ -37,65 +39,91 @@ Qed.
 
 (* Ludicrous that this is the easiest correct definition to write.
  * Generates substitution functions for every free variable at once. *)
-Fixpoint grand_unified_subst t : list (string * (term -> term)) :=
+Fixpoint grand_unified_subst t : option (list (string * hole)) :=
   match t with
   | TmVoid
   | TmStar _
   | TmAtom _ =>
-      []
+      Some []
   | TmVarS s =>
-      [(s, fun x => x)]
+      Some [(s, HoleHere)]
   | TmPack id arg ty curry =>
-      let lo := smap (fun f x => TmPack id arg ty (f x)) (
-        let recursed := grand_unified_subst curry in
-        match arg with
-        | None => recursed
-        | Some a => remove_key_if_head a recursed
-        end) in
-      let hi := smap (fun f x => TmPack id arg (f x) curry) (structural_grand_unified_subst ty) in
-      partition_pf fst_cmp hi lo ++ lo
+      match grand_unified_subst curry with
+      | None => None
+      | Some recursed =>
+        let lo := smap (HolePackCurry id arg ty) (
+          match arg with
+          | None => recursed
+          | Some a => remove_key_if_head a recursed
+          end) in
+        let hi := smap (fun h => HolePackTy id arg h curry) (structural_grand_unified_subst ty) in
+        option_map (fun li => li ++ lo) (partition_kv_pf eqb eq_hole hi lo)
+      end
   | TmForA arg ty body =>
-      let lo := smap (fun f x => TmForA arg ty (f x)) (
-        let recursed := grand_unified_subst body in
-        match arg with
-        | None => recursed
-        | Some a => remove_key_if_head a recursed
-        end) in
-      let hi := smap (fun f x => TmForA arg (f x) body) (structural_grand_unified_subst ty) in
-      partition_pf fst_cmp hi lo ++ lo
-  | TmAppl a b =>
-      smap (fun f x => TmAppl (f x) b) (grand_unified_subst a) ++
-      smap (fun f x => TmAppl a (f x)) (grand_unified_subst b)
+      match grand_unified_subst body with
+      | None => None
+      | Some recursed =>
+        let lo := smap (HoleForABody arg ty) (
+          match arg with
+          | None => recursed
+          | Some a => remove_key_if_head a recursed
+          end) in
+        let hi := smap (fun h => HoleForATy arg h body) (structural_grand_unified_subst ty) in
+        option_map (fun li => li ++ lo) (partition_kv_pf eqb eq_hole hi lo)
+      end
+  | TmAppl f x =>
+      match grand_unified_subst f, grand_unified_subst x with
+      | Some sf, Some sx => Some (smap (fun h => HoleApplF h x) sf ++ smap (HoleApplX f) sx)
+      | _, _ => None
+      end
   end.
 
-Definition subst x y t := option_map (fun f => f y) (pair_lookup x (grand_unified_subst t)).
+Definition subst x y t :=
+  match grand_unified_subst t with
+  | None => None
+  | Some s => option_map (fun f => fill f y) (pair_lookup x s)
+  end.
 Arguments subst x y t/.
 
 Example subst_simple : forall f x,
-  subst f TmVoid (TmAppl (TmVarS f) x) = Some (TmAppl TmVoid x).
+  subst f TmVoid (TmAppl (TmVarS f) (TmVarS x)) = Some (TmAppl TmVoid (TmVarS x)).
 Proof. intros. simpl. rewrite eqb_refl. reflexivity. Qed.
 
 Example grand_unified_subst_simple :
-  grand_unified_subst (TmAppl (TmVarS "f"%string) (TmVarS "x"%string)) = [
-    ("f"%string, fun t => TmAppl t (TmVarS "x"%string));
-    ("x"%string, fun t => TmAppl (TmVarS "f"%string) t)].
+  grand_unified_subst (TmAppl (TmVarS "f"%string) (TmVarS "x"%string)) = Some [
+    ("f", HoleApplF HoleHere (TmVarS "x"));
+    ("x", HoleApplX (TmVarS "f") HoleHere)]%string.
 Proof. reflexivity. Qed.
 
 Example grand_unified_subst_lambda :
-  grand_unified_subst (TmForA (Some "x") (TmVarS "T") (TmAppl (TmVarS "x") (TmVarS "x")))%string = [
-    ("T", fun x => TmForA (Some "x") x (TmAppl (TmVarS "x") (TmVarS "x")));
+  grand_unified_subst (TmForA (Some "x") (TmVarS "T") (TmAppl (TmVarS "x") (TmVarS "x")))%string = Some [
+    ("T", HoleForATy (Some "x") HoleHere (TmAppl (TmVarS "x") (TmVarS "x")));
     (* ignore the first `x`, since it's bound, then *)
-    ("x", fun x => TmForA (Some "x") (TmVarS "T") (TmAppl (TmVarS "x") x))]%string.
+    ("x", HoleForABody (Some "x") (TmVarS "T") (HoleApplX (TmVarS "x") HoleHere))]%string.
 Proof. reflexivity. Qed.
 
 Lemma fst_cmp_eqb : forall {T} a a' b b',
   @fst_cmp T T (a, b) (a', b') = eqb a a'.
 Proof. reflexivity. Qed.
 
-Theorem grand_unified_subst_fv : forall t,
-  fv t = map fst (grand_unified_subst t).
+Theorem grand_unified_subst_fv : forall t s,
+  grand_unified_subst t = Some s ->
+  fv t = map fst s.
 Proof.
-  induction t; intros; simpl in *; try reflexivity; repeat rewrite slow_down; repeat rewrite <- partition_pf_fast_slow;
+  induction t; intros; simpl in *; try solve [invert H; reflexivity]; repeat rewrite slow_down in *;
+  repeat rewrite structural_grand_unified_subst_fv in *.
+  - destruct (grand_unified_subst t2) as [s2 |] eqn:Es2; [| discriminate H].
+    specialize (IHt2 _ eq_refl). repeat rewrite IHt2 in *. rewrite slow_down_kv in H.
+    destruct (partition_kv_pf_slow eqb eq_hole
+      (smap (fun h : hole => HolePackTy id arg h t2) (structural_grand_unified_subst t1))
+      (smap (HolePackCurry id arg t1) match arg with Some a => remove_key_if_head a s2 | None => s2 end)
+    ) eqn:Ep; invert H; simpl in *. rewrite <- partition_kv_pf_fast_slow in Ep. eapply partition_kv_pf_works in Ep.
+    Search (PartitionKV _ _ _ -> _).
+    destruct arg. 2: {
+      rewrite <- partition_pf_fast_slow. rewrite <- (map_fst_partition_pf _ _ _ _ fst_cmp_eqb).
+      rewrite map_distr. rewrite map_fst_smap. f_equal. Search fst_cmp.
+    Search partition_pf.
+    clear H.
   rewrite map_distr; try rewrite (map_fst_partition_pf _ _ _ _ fst_cmp_eqb); repeat rewrite map_fst_smap;
   repeat rewrite IHt1; repeat rewrite IHt2; [| | reflexivity]; rewrite structural_grand_unified_subst_fv;
   (destruct arg; [| reflexivity]); repeat rewrite partition_pf_fast_slow; (destruct (grand_unified_subst t2); [reflexivity |]);
@@ -120,16 +148,16 @@ Proof.
 Qed.
 
 Theorem grand_unified_subst_id : forall t,
-  let P := fun p : _ * _ => let (x, f) := p in f (TmVarS x) = t in
+  let P := fun p : _ * _ => let (x, f) := p in fill f (TmVarS x) = t in
   Forall P (grand_unified_subst t).
 Proof.
   induction t as [| | | | id arg a IHa b IHb | arg a IHa b IHb | a IHa b IHb]; simpl in *; repeat constructor; [| |
     apply Forall_app; split; apply Forall_smap; (eapply Forall_impl; [| try apply IHa; apply IHb]);
-    intros; destruct a0; rewrite H; reflexivity]; repeat rewrite slow_down; destruct arg;
+    intros; destruct a0; simpl; rewrite H; reflexivity]; repeat rewrite slow_down; destruct arg;
   apply Forall_app; (split; [eapply incl_Forall; [apply incl_partition_pf_fst |] |]);
   apply Forall_smap; try (eapply incl_Forall; [apply remove_key_if_head_incl |]);
   (eapply Forall_impl; [| try apply structural_grand_unified_subst_id; apply IHb]);
-  intros; destruct a0; rewrite H; reflexivity.
+  intros; destruct a0; simpl; rewrite H; reflexivity.
 Qed.
 
 Theorem subst_id : forall x t s,
@@ -138,4 +166,76 @@ Theorem subst_id : forall x t s,
 Proof.
   intros. unfold subst in *. destruct (pair_lookup x (grand_unified_subst t)) eqn:Ep; invert H.
   eapply pair_lookup_Forall in Ep; [| apply grand_unified_subst_id]. assumption.
+Qed.
+
+Variant DecapitateK {K V} (k : K) : list (K * V) -> list (K * V) -> Prop :=
+  | DecapitateKNil :
+      DecapitateK k [] []
+  | DecapitateKConsEq : forall hv tl,
+      DecapitateK k ((k, hv) :: tl) tl
+  | DecapitateKConsNEq : forall hk hv tl,
+      k <> hk ->
+      DecapitateK k ((hk, hv) :: tl) ((hk, hv) :: tl)
+  .
+
+Theorem reflect_decapitate_k : forall {V} k li post,
+  remove_key_if_head k li = post <-> @DecapitateK _ V k li post.
+Proof.
+  split; intros.
+  - subst. destruct li; simpl in *. { constructor. }
+    destruct p. destruct (eqb_spec k s). { subst. constructor. } constructor. assumption.
+  - destruct H; simpl in *; [| rewrite eqb_refl | apply eqb_neq in H; rewrite H]; reflexivity.
+Qed.
+
+Inductive GrandUnifiedSubst : term -> list (string * hole) -> Prop :=
+  | GUSVoid :
+      GrandUnifiedSubst TmVoid []
+  | GUSStar : forall univ,
+      GrandUnifiedSubst (TmStar univ) []
+  | GUSVarS : forall s,
+      GrandUnifiedSubst (TmVarS s) [(s, HoleHere)]
+  | GUSAtom : forall id,
+      GrandUnifiedSubst (TmAtom id) []
+  | GUSPack : forall id arg ty curry sty scurry scurry_orig pf s,
+      GrandUnifiedSubst ty sty ->
+      GrandUnifiedSubst curry scurry_orig ->
+      match arg with
+      | None => eq
+      | Some a => DecapitateK a
+      end scurry_orig scurry ->
+      PartitionKV pf sty scurry ->
+      s = smap (fun h => HolePackTy id arg h curry) pf ++ smap (HolePackCurry id arg ty) scurry ->
+      GrandUnifiedSubst (TmPack id arg ty curry) s
+  | GUSForA : forall arg ty body sty sbody sbody_orig pf s,
+      GrandUnifiedSubst ty sty ->
+      GrandUnifiedSubst body sbody_orig ->
+      match arg with
+      | None => eq
+      | Some a => DecapitateK a
+      end sbody_orig sbody ->
+      PartitionKV pf sty sbody ->
+      s = smap (fun h => HoleForATy arg h body) pf ++ smap (HoleForABody arg ty) sbody ->
+      GrandUnifiedSubst (TmForA arg ty body) s
+  | GUSAppl : forall f x sf sx s,
+      GrandUnifiedSubst f sf ->
+      GrandUnifiedSubst x sx ->
+      s = smap (fun h => HoleApplF h x) sf ++ smap (HoleApplX f) sx ->
+      GrandUnifiedSubst (TmAppl f x) s
+  .
+
+Theorem reflect_structural_grand_unified_subst : forall t s,
+  grand_unified_subst t = s <-> GrandUnifiedSubst t s.
+Proof.
+  split; intros.
+  - generalize dependent s. induction t; intros; subst; simpl in *; try solve [constructor]; try rewrite slow_down.
+    + econstructor.
+      * apply IHt1. reflexivity.
+      * apply IHt2. reflexivity.
+      * shelve.
+      * apply (partition_pf_works). Search (partition_pf).
+      * f_equal.
+
+    econstructor. ; try apply IHt1; try apply IHt2; try reflexivity; (destruct arg; [apply reflect_purge_k |]); reflexivity.
+  - induction H; subst; simpl in *; f_equal; (destruct arg; [| subst; reflexivity]);
+    apply reflect_purge_k in H1; subst; reflexivity.
 Qed.
