theories/StructuralHole.v
@@ -1,0 +1,94 @@
+From Lang Require Import
+  Hole
+  Invert
+  Terms.
+
+Inductive structural_hole : Set :=
+  | SHoleHere
+  | SHoleTerm (tm : term)
+  | SHolePack (id : string) (arg : option string) (ty : structural_hole) (curry : structural_hole)
+  | SHoleForA (arg : option string) (ty : structural_hole) (body : structural_hole)
+  | SHoleAppl (f : structural_hole) (x : structural_hole)
+  .
+
+Fixpoint sfill h t : term :=
+  match h with
+  | SHoleHere => t
+  | SHoleTerm tm => tm
+  | SHolePack id arg ty curry => TmPack id arg (sfill ty t) (sfill curry t)
+  | SHoleForA arg ty body => TmForA arg (sfill ty t) (sfill body t)
+  | SHoleAppl f x => TmAppl (sfill f t) (sfill x t)
+  end.
+
+Inductive StructuralFill : structural_hole -> term -> term -> Prop :=
+  | SFillHere : forall t,
+      StructuralFill SHoleHere t t
+  | SFillNone : forall t tm,
+      StructuralFill (SHoleTerm tm) t tm
+  | SFillPack : forall t id arg ty curry ty' curry',
+      StructuralFill ty t ty' ->
+      StructuralFill curry t curry' ->
+      StructuralFill (SHolePack id arg ty curry) t (TmPack id arg ty' curry')
+  | SFillForA : forall t arg ty body ty' body',
+      StructuralFill ty t ty' ->
+      StructuralFill body t body' ->
+      StructuralFill (SHoleForA arg ty body) t (TmForA arg ty' body')
+  | SFillAppl : forall t f x f' x',
+      StructuralFill f t f' ->
+      StructuralFill x t x' ->
+      StructuralFill (SHoleAppl f x) t (TmAppl f' x')
+  .
+
+Theorem reflect_sfill : forall h t t',
+  sfill h t = t' <-> StructuralFill h t t'.
+Proof.
+  split; intros.
+  - generalize dependent t. generalize dependent t'.
+    induction h; intros; subst; simpl in *; constructor; try apply IHh1; try apply IHh2; reflexivity.
+  - induction H; simpl in *; try rewrite IHStructuralFill1; try rewrite IHStructuralFill2; reflexivity.
+Qed.
+
+Fixpoint eq_shole a b :=
+  match a, b with
+  | SHoleHere, SHoleHere =>
+      true
+  | SHoleTerm ta, SHoleTerm tb =>
+      eq_term ta tb
+  | SHolePack ida arga tya currya, SHolePack idb argb tyb curryb =>
+      andb (eqb ida idb) (andb (eq_opt arga argb) (andb (eq_shole tya tyb) (eq_shole currya curryb)))
+  | SHoleForA arga tya currya, SHoleForA argb tyb curryb =>
+      andb (eq_opt arga argb) (andb (eq_shole tya tyb) (eq_shole currya curryb))
+  | SHoleAppl fa xa, SHoleAppl fb xb =>
+      andb (eq_shole fa fb) (eq_shole xa xb)
+  | _, _ => false
+  end.
+
+Theorem eq_shole_spec : forall a b,
+  Bool.reflect (a = b) (eq_shole a b).
+Proof.
+  induction a; intros []; simpl in *; try solve [constructor; try reflexivity; try (intro C; discriminate C)];
+  try (destruct (eq_term_spec tm tm0); [| rf n]);
+  try (destruct (eqb_spec id id0); [| rf n]);
+  try (destruct (eq_opt_spec arg arg0); [| rf n]);
+  try (destruct (IHa1 ty); [| rf n]);
+  try (destruct (IHa2 curry); [| rf n]);
+  try (destruct (IHa2 body); [| rf n]);
+  try (destruct (IHa1 f); [| rf n]);
+  try (destruct (IHa2 x); [| rf n]);
+  constructor; subst; reflexivity.
+Qed.
+
+Fixpoint structuralize h :=
+  match h with
+  | HoleHere => SHoleHere
+  | HolePackTy id arg ty curry => SHolePack id arg (structuralize ty) (SHoleTerm curry)
+  | HolePackCurry id arg ty curry => SHolePack id arg (SHoleTerm ty) (structuralize curry)
+  | HoleForATy arg ty body => SHoleForA arg (structuralize ty) (SHoleTerm body)
+  | HoleForABody arg ty body => SHoleForA arg (SHoleTerm ty) (structuralize body)
+  | HoleApplF f x => SHoleAppl (structuralize f) (SHoleTerm x)
+  | HoleApplX f x => SHoleAppl (SHoleTerm f) (structuralize x)
+  end.
+
+Theorem structuralize_invariant : forall h t,
+  fill h t = sfill (structuralize h) t.
+Proof. induction h; intros; simpl in *; try rewrite IHh; reflexivity. Qed.
